More Blake2 wrappers

code/hash/Hacl.Hash.Blake2.fst
@@ -3,12 +3,16 @@ module Hacl.Hash.Blake2
 module B = LowStar.Buffer
 module ST = FStar.HyperStack.ST
 module BlB32 = Hacl.Blake2b_32
+module BlS32 = Hacl.Blake2s_32
+module BlS128 = Hacl.Blake2s_128
 open Lib.IntTypes
 open Lib.Buffer
 
 #push-options "--fuel 0 --ifuel 0 --z3rlimit 20"
 
 friend Spec.Agile.Hash
+
+// Blake2b_32
 
 let alloca_blake2b_32 () =
   let h0 = ST.get() in
@@ -34,3 +38,59 @@ let update_last_blake2b_32 s prev input input_len =
   ST.pop_frame()
 
 let finish_blake2b_32 s dst = BlB32.blake2b_finish (hash_len Blake2B) dst s
+
+
+// Blake2s_32
+
+let alloca_blake2s_32 () =
+  let h0 = ST.get() in
+  let s = Hacl.Impl.Blake2.Core.alloc_state Spec.Blake2.Blake2S M32 in
+  BlS32.blake2s_init s 0ul 32ul;
+  let h1 = ST.get () in
+  B.modifies_only_not_unused_in (B.loc_none) h0 h1;
+  assert (B.modifies B.loc_none h0 h1);
+  s
+
+let init_blake2s_32 s = BlS32.blake2s_init s 0ul 32ul
+
+let update_multi_blake2s_32 s ev blocks n =
+  ST.push_frame ();
+  let wv = Hacl.Impl.Blake2.Core.alloc_state Spec.Blake2.Blake2S M32 in
+  BlS32.blake2s_update_multi #(n `FStar.UInt32.mul` block_len Blake2S) wv s ev blocks n;
+  ST.pop_frame ()
+
+let update_last_blake2s_32 s prev input input_len =
+  ST.push_frame ();
+  let wv = Hacl.Impl.Blake2.Core.alloc_state Spec.Blake2.Blake2S M32 in
+  BlS32.blake2s_update_last #input_len wv s (secret prev) input_len input;
+  ST.pop_frame()
+
+let finish_blake2s_32 s dst = BlS32.blake2s_finish (hash_len Blake2S) dst s
+
+
+// Blake2s_128
+
+let alloca_blake2s_128 () =
+  let h0 = ST.get() in
+  let s = Hacl.Impl.Blake2.Core.alloc_state Spec.Blake2.Blake2S M128 in
+  BlS128.blake2s_init s 0ul 32ul;
+  let h1 = ST.get () in
+  B.modifies_only_not_unused_in (B.loc_none) h0 h1;
+  assert (B.modifies B.loc_none h0 h1);
+  s
+
+let init_blake2s_128 s = BlS128.blake2s_init s 0ul 32ul
+
+let update_multi_blake2s_128 s ev blocks n =
+  ST.push_frame ();
+  let wv = Hacl.Impl.Blake2.Core.alloc_state Spec.Blake2.Blake2S M128 in
+  BlS128.blake2s_update_multi #(n `FStar.UInt32.mul` block_len Blake2S) wv s ev blocks n;
+  ST.pop_frame ()
+
+let update_last_blake2s_128 s prev input input_len =
+  ST.push_frame ();
+  let wv = Hacl.Impl.Blake2.Core.alloc_state Spec.Blake2.Blake2S M128 in
+  BlS128.blake2s_update_last #input_len wv s (secret prev) input_len input;
+  ST.pop_frame()
+
+let finish_blake2s_128 s dst = BlS128.blake2s_finish (hash_len Blake2S) dst s
